lemmas in wp_codegen, kinding ftlr work

theories/iris/wp_codegen.v
@@ -65,7 +65,110 @@ Section CodeGen.
     iSimpl.
     iDestruct "Hbl" as "[[%Hi Hbl] | [%Hi Hbl]]".
     - by iApply (wp_if_true with "[Hfr] [Hrun]"); auto.
-    - by iApply (wp_if_false with "[Hfr] [Hrun]"); auto.
+     - by iApply (wp_if_false with "[Hfr] [Hrun]"); auto.
   Qed.
+
+  (* Generic monad operations. *)
+  Lemma wp_ret {A} (a: A) wl v wl' es :
+    run_codegen (Monad.ret a) wl = inr (v, wl', es) ->
+    v = a /\ wl' = wl /\ es = [].
+  Proof.
+    cbn.
+    intros Hcg.
+    inversion Hcg; subst; done.
+  Qed.
+
+  Lemma wp_mapM_nil {A B} (f: A -> codegen (list B)) wl ys wl' es :
+    run_codegen (mapM f []) wl = inr (ys, wl', es) ->
+    wl' = wl /\
+    ys = [] /\
+    es = [].
+  Proof.
+    cbn.
+    intros Hcg.
+    inversion Hcg.
+    done.
+  Qed.
+  
+  Lemma wp_mapM_cons {A B} (f: A -> codegen (list B)) wl yss wl' es x xs :
+    run_codegen (mapM f (x :: xs)) wl = inr (yss, wl', es) ->
+    ∃ ys_x wl_x es_x yss_xs wl_xs es_xs,
+      run_codegen (f x) wl = inr (ys_x, wl_x, es_x) /\
+      run_codegen (mapM f xs) wl_x = inr (yss_xs, wl_xs, es_xs) /\
+      yss = ys_x :: yss_xs /\
+      wl' = wl_xs /\
+      es = es_x ++ es_xs.
+  Proof.
+    cbn.
+    intros Hcg.
+    inv_cg_bind Hcg res1 wl1 es_fx es2 Hfx Hcg1.
+    inv_cg_bind Hcg1 res2 wl2 es_fxs es3 Hfxs Hcg2.
+    cbn in Hcg2.
+    inversion Hcg2.
+    subst.
+    repeat eexists; eauto.
+    rewrite app_nil_r; eauto.
+  Qed.
+
+  (* State monad operations. *) 
+  Lemma wp_get wl v wl' es :
+    run_codegen MonadState.get wl = inr (v, wl', es) ->
+    v = wl /\
+    wl' = wl /\
+    es = [].
+  Proof.
+    unfold MonadState.get; cbn.
+    intros Heq.
+    inversion Heq; subst.
+    tauto.
+  Qed.
+
+  Lemma wp_put wl v wl' wl'' es :
+    run_codegen (MonadState.put wl') wl = inr (v, wl'', es) ->
+    v = () /\
+    wl'' = wl' /\
+    es = [].
+  Proof.
+    unfold MonadState.put; cbn.
+    intros Heq.
+    inversion Heq; subst.
+    tauto.
+  Qed.
+  
+  (* Allocating locals. *)
+  
+  (* Monotone interpretation of a wlocal_ctx *)
+  Definition interp_wl (wlocal_offset : nat) (wl : wlocal_ctx) (inst: instance) : frame -> Prop :=
+    λ fr, ∃ vs vs__wl vs', fr = Build_frame (vs ++ vs__wl ++ vs') inst /\
+                         result_type_interp wl vs__wl.
+
+  Lemma wp_wlalloc fe ty wl wl' idx es :
+    run_codegen (wlalloc fe ty) wl = inr (idx, wl', es) ->
+    idx = Mk_localidx (fe_wlocal_offset fe + length wl) /\
+    wl' = wl ++ [ty] /\
+    es = [].
+  Proof.
+    unfold wlalloc.
+    intros Hcg.
+    inv_cg_bind Hcg res wl1 es_get es2 Hget Hcg1.
+    inv_cg_bind Hcg1 res1 wl2 es_put es_ret Hput Hret.
+    apply wp_get in Hget.
+    apply wp_put in Hput.
+    apply wp_ret in Hret.
+    destruct Hget as (? & ? & ?).
+    destruct Hput as (? & ? & ?).
+    destruct Hret as (? & ? & ?).
+    subst; done.
+  Qed.
+
+  (* Saving and restoring the stack. *)
+  Lemma wp_save_stack_w s E Φ inst fe ty wl idx wl' es fr :
+    run_codegen (save_stack_w fe ty) wl = inr (idx, wl', es) ->
+    interp_wl (fe_wlocal_offset fe) wl' inst fr ->
+    ⊢ ↪[frame] fr -∗
+      ↪[RUN] -∗
+      WP (to_e_list es) @ s; E {{ v, Φ v }}.
+  Abort.
+
 
 End CodeGen.
